module weak-normalization where

record _*_ (A B : Set) : Set where
 constructor _,_
 field
  fst : A
  snd : B

record Σ {A : Set} (B : A -> Set) : Set where
 constructor _,_
 field
  fst : A
  snd : B fst

data _≡_ {A : Set} (x : A) : A -> Set where
 refl : x ≡ x

{-# BUILTIN EQUALITY _≡_ #-}
{-# BUILTIN REFL refl #-}

postulate
 funext : ∀ {A} {B : A -> Set} {f g : (x : A) -> B x} -> (∀ x -> f x ≡ g x) -> f ≡ g
 funext-imp : ∀ {A : Set} {B : A -> Set} {f g : (x : A) -> B x} -> (∀ x -> f x ≡ g x) -> _≡_ { {x : A} -> B x} (λ {x} -> f x) (λ {x} -> g x)

cong-app1 : ∀ {A} {B : A -> Set} {f g : (x : A) -> B x} -> f ≡ g -> (x : A) -> f x ≡ g x
cong-app1 refl x = refl

cong-app : ∀ {A B : Set} {f g : A -> B} -> f ≡ g -> {x y : A} -> x ≡ y -> f x ≡ g y
cong-app refl refl = refl 

cong : ∀ {A B : Set} (f : A -> B) {x y : A} -> x ≡ y -> f x ≡ f y
cong f refl = refl

cong1/2 : ∀ {A B C : Set} (f : A -> B -> C) -> {x y : A} -> x ≡ y -> (z : B) -> f x z ≡ f y z
cong1/2 f refl z = refl 

cong2 : ∀ {A B C : Set} (f : A -> B -> C) -> {x y : A} -> x ≡ y -> {z w : B} -> z ≡ w -> f x z ≡ f y w
cong2 f refl refl = refl

eq-ind : ∀ {A} (P : A -> Set) -> {x y : A} -> x ≡ y -> P x -> P y
eq-ind P refl t = t 

eq-ind2 : ∀ {A B} (P : A -> B -> Set) -> {x y : A} -> x ≡ y -> {z w : B} -> z ≡ w -> P x z -> P y w
eq-ind2 P refl refl t = t

eq-sub1 : ∀ {A C} (P : A -> C) {t} -> {x y : A} -> x ≡ y -> P y ≡ t -> P x ≡ t
eq-sub1 P refl p = p 

eq-sub2 : ∀ {A B C} (P : A -> B -> C) {t} -> {x y : A} -> x ≡ y -> {z w : B} -> z ≡ w -> P y w ≡ t -> P x z ≡ t
eq-sub2 P refl refl p = p

trans : ∀ {A} {x y z : A} -> x ≡ y -> y ≡ z -> x ≡ z
trans refl refl = refl

sym : ∀ {A} {x y : A} -> x ≡ y -> y ≡ x
sym refl = refl

record Unit : Set where
 constructor tt

postulate
 atomic_tp : Set

data tp : Set where
 atom : (A : atomic_tp) -> tp
 _⇝_ : (T : tp) -> (S : tp) -> tp

data ctx : Set where
 ⊡ : ctx
 _,_ : (Γ : ctx) -> (T : tp) -> ctx

data var : (Γ : ctx) -> (T : tp) -> Set where
 z : ∀ {Γ T} -> var (Γ , T) T
 s : ∀ {Γ T S} -> var Γ T -> var (Γ , S) T

vsubst : ctx -> ctx -> Set 
vsubst Δ Γ = ∀ {U} -> var Δ U -> var Γ U

mutual 
 data rtm (Γ : ctx) : (T : tp) -> Set where
  v : ∀ {T} -> var Γ T -> rtm Γ T
  _·_ : ∀ {T S} -> rtm Γ (T ⇝ S) -> ntm Γ T -> rtm Γ S
 data ntm (Γ : ctx) : (T : tp) -> Set where
  ƛ : ∀ {T S} -> ntm (Γ , T) S -> ntm Γ (T ⇝ S)
  neut : ∀ {A} -> rtm Γ (atom A) -> ntm Γ (atom A)


{-sem : (Γ : ctx) -> (T : tp) -> Set
sem Γ (atom A) = ntm Γ (atom A)
sem Γ (T ⇝ S) = ∀ Δ -> vsubst Γ Δ -> sem Δ T → sem Δ S -}

_∘_ : ∀ {Δ Γ ψ} -> vsubst Δ Γ -> vsubst ψ Δ -> vsubst ψ Γ
(σ1 ∘ σ2) x = σ1 (σ2 x)

_∘₁_ : ∀ {A B C : Set} (f : B -> C) (g : A -> B) -> A -> C
(f ∘₁ g) x = f (g x)

ext : ∀ {Γ Δ T} -> vsubst Γ Δ -> vsubst (Γ , T) (Δ , T)
ext σ z = z
ext σ (s y) = s (σ y)

mutual
 rappSubst : ∀ {Γ Δ S} -> vsubst Δ Γ -> rtm Δ S -> rtm Γ S
 rappSubst σ (v y) = v (σ y)
 rappSubst σ (R · N) = rappSubst σ R · nappSubst σ N
 nappSubst : ∀ {Γ Δ S} -> vsubst Δ Γ -> ntm Δ S -> ntm Γ S 
 nappSubst σ (ƛ M) = ƛ (nappSubst (ext σ) M)
 nappSubst σ (neut R) = neut (rappSubst σ R)


var-dom-eq' : ∀ {A : tp -> Set} {Γ T} (f g : ∀ {U} (x : var (Γ , T) U) -> A U) -> (∀ {U} (x : var Γ U) -> f (s x) ≡ g (s x)) -> f z ≡ g z -> ∀ {U} (x : var (Γ , T) U) -> f x ≡ g x
var-dom-eq' f g p q z = q
var-dom-eq' f g p q (s y) = p y

var-dom-eq : ∀ {A : tp -> Set} {Γ T} {f g : ∀ {U} (x : var (Γ , T) U) -> A U} -> (∀ {U} (x : var Γ U) -> f (s x) ≡ g (s x)) -> f z ≡ g z -> _≡_ { ∀ {U} -> var (Γ , T) U -> A U } f g
var-dom-eq {f = f} {g = g} p q = funext-imp (λ U -> funext (λ x -> var-dom-eq' f g p q x))

ext-funct : ∀ {Γ1 Γ2 Γ3 U S} (σ1 : vsubst Γ2 Γ3) (σ2 : vsubst Γ1 Γ2) (x : var (Γ1 , U) S) -> ((ext σ1) ∘ (ext σ2)) x ≡ ext (σ1 ∘ σ2) x
ext-funct σ1 σ2 z = refl
ext-funct σ1 σ2 (s y) = refl

mutual
 rappSubst-funct : ∀ {Γ1 Γ2 Γ3 S} (σ1 : vsubst Γ2 Γ3) (σ2 : vsubst Γ1 Γ2) (R : rtm Γ1 S)
  -> rappSubst σ1 (rappSubst σ2 R) ≡ rappSubst (σ1 ∘ σ2) R
 rappSubst-funct σ1 σ2 (v y) = refl
 rappSubst-funct σ1 σ2 (R · N) = cong2 _·_ (rappSubst-funct σ1 σ2 R) (nappSubst-funct σ1 σ2 N)
 nappSubst-funct : ∀ {Γ1 Γ2 Γ3 S} (σ1 : vsubst Γ2 Γ3) (σ2 : vsubst Γ1 Γ2) (N : ntm Γ1 S)
  -> nappSubst σ1 (nappSubst σ2 N) ≡ nappSubst (σ1 ∘ σ2) N
 nappSubst-funct σ1 σ2 (ƛ N) = cong ƛ (trans (nappSubst-funct (ext σ1) (ext σ2) N) (cong (λ (α : vsubst _ _) → nappSubst α N) (funext-imp (λ U → funext (λ x' → ext-funct σ1 σ2 x')))))
 nappSubst-funct σ1 σ2 (neut R) = cong neut (rappSubst-funct σ1 σ2 R)

id : ∀ {Γ} -> vsubst Γ Γ
id x = x

ext-id : ∀ {Γ T U} (x : var (Γ , T) U) -> ext id x ≡ x
ext-id z = refl
ext-id (s y) = refl

mutual
 rappSubst-id : ∀ {Γ S} (R : rtm Γ S) -> rappSubst id R ≡ R
 rappSubst-id (v y) = refl
 rappSubst-id (R · N) = cong2 _·_ (rappSubst-id R) (nappSubst-id N)
 nappSubst-id : ∀ {Γ S} (N : ntm Γ S) -> nappSubst id N ≡ N
 nappSubst-id (ƛ N) = cong ƛ (trans (cong (λ (α : vsubst _ _) → nappSubst α N) (funext-imp (λ U → funext (λ x → ext-id x)))) (nappSubst-id N))
 nappSubst-id (neut R) = cong neut (rappSubst-id R)

{-
appSubst : ∀ {Γ Δ} S -> vsubst Δ Γ -> sem Δ S -> sem Γ S
appSubst (atom A) σ M = nappSubst σ M
appSubst (T ⇝ S) σ M = λ _ σ' s → M _ (σ' ∘ σ) s -}

wkn : ∀ {Γ T} -> vsubst Γ (Γ , T)
wkn = s

{-
mutual
 reflect : ∀ {T Γ} -> rtm Γ T -> sem Γ T
 reflect {atom A} N = neut N
 reflect {T ⇝ S} N = λ _ σ s → reflect (rappSubst σ N · reify s)

 reify : ∀ {T Γ} -> sem Γ T -> ntm Γ T
 reify {atom A} M = M
 reify {T ⇝ S} M = ƛ (reify (M _ wkn (reflect (v z))))

subst : ctx -> ctx -> Set
subst Γ Δ = ∀ {T} -> var Γ T -> sem Δ T

extend : ∀ {Γ Δ T} -> subst Γ Δ -> sem Δ T -> subst (Γ , T) Δ
extend θ M z = M
extend θ M (s y) = θ y
-}
data tm (Γ : ctx) : (T : tp) -> Set where
 v : ∀ {T} -> var Γ T -> tm Γ T
 _·_ : ∀ {T S} -> tm Γ (T ⇝ S) -> tm Γ T -> tm Γ S
 ƛ : ∀ {T S} -> tm (Γ , T) S -> tm Γ (T ⇝ S)

{-
_◦_ : ∀ {Γ1 Γ2 Γ3} -> vsubst Γ2 Γ3 -> subst Γ1 Γ2 -> subst Γ1 Γ3
(σ ◦ θ) = λ x ->  appSubst _ σ (θ x)


-- Traditional nbe
-- This is taking tm Γ T into a Yoneda-like Hom space
eval : ∀ {Γ Δ T} -> subst Γ Δ -> tm Γ T -> sem Δ T
eval θ (v y) = θ y
eval θ (M · N) = eval θ M _ id (eval θ N)
eval θ (ƛ M) = λ _ σ s -> eval (extend (σ ◦ θ) s) M


nbe : ∀ {Γ T} -> tm Γ T -> ntm Γ T
nbe M = reify (eval (λ x → reflect (v x)) M)
-}

[_]v : ∀ {Γ1 Γ2 T} (σ : vsubst Γ1 Γ2) -> (M : tm Γ1 T) -> tm Γ2 T
[_]v σ (v y) = v (σ y)
[_]v σ (M · N) = [ σ ]v M · [ σ ]v N
[_]v σ (ƛ M) = ƛ ([ ext σ ]v M)

sub : (Γ1 Γ2 : ctx) -> Set
sub Γ1 Γ2 = ∀ {T} -> var Γ1 T -> tm Γ2 T

sub-ext : ∀ {Γ1 Γ2 T} -> sub Γ1 Γ2 -> sub (Γ1 , T) (Γ2 , T)
sub-ext σ z = v z
sub-ext σ (s y) = [ s ]v (σ y)

[_] : ∀ {Γ1 Γ2 T} (σ : sub Γ1 Γ2) -> (M : tm Γ1 T) -> tm Γ2 T
[_] σ (v y) = σ y
[_] σ (M · N) = [ σ ] M · [ σ ] N
[_] σ (ƛ M) = ƛ ([ sub-ext σ ] M)

_,,_ : ∀ {Γ1 Γ2 T} -> sub Γ1 Γ2 -> tm Γ2 T -> sub (Γ1 , T) Γ2
(σ ,, M) z = M
(σ ,, M) (s y) = σ y

-- Why not just use an explicit substitution calculus?
data _→*_ {Γ} : ∀ {T} -> tm Γ T -> tm Γ T -> Set where
 v : ∀ {T} (x : var Γ T) -> (v x) →* (v x)
 _·_ : ∀ {T S} {M1 M2 : tm Γ (T ⇝ S)} {N1 N2 : tm Γ T} -> M1 →* M2 -> N1 →* N2 -> (M1 · N1) →* (M2 · N2)
 ƛ : ∀ {T S} {M1 M2 : tm (Γ , T) S} -> M1 →* M2 -> (ƛ M1) →* (ƛ M2)
 β : ∀ {T S} (M : tm (Γ , T) S) (N : tm Γ T) -> ((ƛ M) · N) →* [ v ,, N ] M
-- η : ∀ {T S} (M : tm Γ (T ⇝ S)) -> M →* (ƛ ([ s ]v M · (v z)))
 →*-trans : ∀ {T} {M N P : tm Γ T} -> M →* N -> N →* P -> M →* P

→*-refl : ∀ {Γ T} {M : tm Γ T} -> M →* M
→*-refl {M = v y} = v y
→*-refl {M = M · N} = →*-refl · →*-refl
→*-refl {M = ƛ M} = ƛ →*-refl

mutual
 ninj : ∀ {Γ T} -> ntm Γ T -> tm Γ T
 ninj (ƛ M) = ƛ (ninj M)
 ninj (neut R) = rinj R
 rinj : ∀ {Γ T} -> rtm Γ T -> tm Γ T
 rinj (v x) = v x
 rinj (R · N) = (rinj R) · (ninj N)


wn : ∀ Γ T -> tm Γ T -> Set
wn Γ (atom A) t = Σ (λ (n : ntm Γ (atom A)) → t →* ninj n)
wn Γ (T ⇝ S) t = ∀ Δ (σ : vsubst Γ Δ) (x : tm Δ T) -> wn Δ T x -> wn Δ S (([ σ ]v t) · x)

wn-closed : ∀ {Γ T} {t t' : tm Γ T} -> (t →* t') -> wn Γ T t' -> wn Γ T t
wn-closed (v x) x' = x'
wn-closed (y · y') x = {!!}
wn-closed (ƛ y) x = {!!}
wn-closed (β M N) x = {!!}
wn-closed (→*-trans y y') x = {!!}

thm : ∀ {Γ Δ T} (σ : ∀ {U} (x : var Γ U) -> tm Δ U) (θ : ∀ {U} (x : var Γ U) -> wn Δ U (σ x)) (t : tm Γ T) -> wn Δ T ([ σ ] t)
thm σ θ (v y) = θ y
thm σ θ (M · N) = eq-ind (wn _ _) (cong2 _·_ {!!} refl) ((thm σ θ M) _ id ([ σ ] N) (thm σ θ N))
thm σ θ (ƛ M) = λ Δ σ' x x' → {!!}
 where f : ∀ Δ (σ' : vsubst _ Δ) (x : tm Δ _) (x' : wn Δ _ x) -> wn Δ _ ([ ([ σ' ]v ∘₁ σ) ,, x ] M)
       f Δ σ' x x' = thm (([ σ' ]v ∘₁ σ) ,, x) {!!} M